specs/Spec.HSalsa20.fst
@@ -4,6 +4,7 @@ open FStar.Mul
 open FStar.Seq
 open FStar.UInt32
 open FStar.Endianness
+open Seq.Create
 open Spec.Lib
 
 let keylen = 32 (* in bytes *)
@@ -21,27 +22,16 @@ type state = Spec.Salsa20.state
 let setup (k:key) (n:nonce): state =
   let ks = uint32s_from_le 8 k in
   let ns = uint32s_from_le 4 n in
-  (set 0  Spec.Salsa20.constant0 @
-   set 5  Spec.Salsa20.constant1 @
-   set 10 Spec.Salsa20.constant2 @
-   set 15 Spec.Salsa20.constant3 @
-   set 1  (index ks 0) @
-   set 2  (index ks 1) @ 
-   set 3  (index ks 2) @ 
-   set 4  (index ks 3) @ 
-   set 11  (index ks 4) @
-   set 12  (index ks 5) @ 
-   set 13  (index ks 6) @ 
-   set 14  (index ks 7) @ 
-   set 6  (index ns 0) @ 
-   set 7  (index ns 1) @ 
-   set 8  (index ns 2) @ 
-   set 9  (index ns 3))
-  (create 16 0ul)
+  let k_fst_half = slice ks 0 4 in
+  let k_snd_half = slice ks 4 8 in
+  let c0 = singleton (Spec.Salsa20.constant0) in
+  let c1 = singleton (Spec.Salsa20.constant1) in
+  let c2 = singleton (Spec.Salsa20.constant2) in
+  let c3 = singleton (Spec.Salsa20.constant3) in
+  c0 @| k_fst_half @| c1 @| ns @| c2 @| k_snd_half @| c3
 
 let hsalsa20 (k:key) (n:nonce) : Tot key = 
   let st = setup k n in
   let st' = Spec.Salsa20.rounds st in
-  let hs = seq_of_list [index st' 0; index st' 5; index st' 10; index st' 15; 
-      	   	        index st' 6; index st' 7; index st' 8; index st' 9] in
+  let hs = create_8 st'.[0] st'.[5] st'.[10] st'.[15] st'.[6] st'.[7] st'.[8] st'.[9] in
   uint32s_to_le 8 hs
